\documentclass[12pt]{exam}
\firstpageheader{Math 4050}{Worksheet \#2}{Name: Sunny Lee}
\usepackage{amsfonts}
\usepackage{amsmath}
\usepackage{amssymb, graphicx, enumerate, mathrsfs}
\begin{document}


\newcommand{\dd}{\textrm{d}}
\newcommand{\NN}{\mathbb N}
\newcommand{\CC}{\mathbb C}
\newcommand{\QQ}{\mathbb Q}
\newcommand{\ZZ}{\mathbb Z}
\newcommand{\RR}{\mathbb R}
\newcommand{\proofdone}{\hfill $\square$}

$f(x) = \frac{e^x}{1+e^x}$
\begin{enumerate}
    \item $\lim_{x\rightarrow \infty} f(x) = \lim_{x\rightarrow \infty} \frac{e^x}{1+e^x}$ 
    By L'opital's rule: 
    $\lim_{x\rightarrow \infty} \frac{e^x}{1+e^x} = \lim_{x\rightarrow \infty} \frac{e^x}{e^x} = 1$
    Thus, the limit is 1. 
    
    \item $\lim_{x\rightarrow -\infty} \frac{e^x}{1+e^x}$ If we plug in negative, 
    we find that the equation looks like: $\lim_{x\rightarrow \infty} \frac{\frac{1}{e^x}}{1+\frac{1}{e^x}}$
    and as this equation goes to infinity, $\frac{1}{e^x}$ is going to go to zero. Thus, 
    $\lim_{x\rightarrow -\infty} \frac{e^x}{1+e^x} = \frac{0}{1 + 0} = 0$

    \item The derivative of $f$ is $\frac{e^x}{e^{2x} + 2e^x + 1}$ Since $e^x$ is never negative, 
    we can conclude that the numerator is never negative, and for the same reason, the denominator 
    is not negative, as we are adding only positive numbers. 
\end{enumerate}


\end{document}